

Rules :

	Scalar :	Vector :
① $z = Wx$	$\frac{\partial L}{\partial x} = \frac{\partial L}{\partial z} \cdot W$ $\frac{\partial L}{\partial W} = x \cdot \frac{\partial L}{\partial z}$	$\begin{bmatrix} z: N \times 1 \\ x: M \times 1 \\ W: N \times M \end{bmatrix}$ $\nabla_x L = (\nabla_z L) W$ $\nabla_W L = x (\nabla_z L)$
② $z = x \odot y$ o: component-wise multiplication		$[x, y, z: N \times 1]$ $\nabla_x L = (\nabla_z L) \odot y^T$ $\nabla_y L = (\nabla_z L) \odot x^T$
③ $z = x + y$	$\frac{\partial L}{\partial x} = \frac{\partial L}{\partial z}$ $\frac{\partial L}{\partial y} = \frac{\partial L}{\partial z}$	$\begin{bmatrix} x, y, z: N \times 1 \\ \nabla_z L: 1 \times N \end{bmatrix}$ $\nabla_x L = \nabla_z L$ $\nabla_y L = \nabla_z L$
④ $z = g(x)$	$\frac{\partial L}{\partial x} = \frac{\partial L}{\partial z} g'(x)$	$\begin{bmatrix} x, z: N \times 1 \\ \nabla_z L: 1 \times N \\ J_{xg}: \text{Jacobian} \end{bmatrix}$ $\nabla_x L = \nabla_z L J_{xg}$ $= \nabla_z L \odot g'(x)^T$
⑤ $z = g(x)$ $y = h(x)$	$\frac{\partial L}{\partial x} = \frac{\partial L}{\partial z} g'(x) + \frac{\partial L}{\partial y} h'(x)$	

- ① $z_t = \sigma(W_{zh} h_{t-1} + W_{zx} x_t)$
- ② $r_t = \sigma(W_{rh} h_{t-1} + W_{rx} x_t)$
- ③ $\tilde{h}_t = \tanh(W_h (r_t \otimes h_{t-1}) + W_x x_t)$
- ④ $h_t = (1 - z_t) \otimes h_{t-1} + z_t \otimes \tilde{h}_t$

$$\text{delta} = \frac{\partial L}{\partial x(l+1, t)} + \frac{\partial L}{\partial h(l, t+1)}$$

$$\Rightarrow \textcircled{1}: z_1 = W_{zh} h_{t-1}$$

$$z_2 = W_{zx} x_t$$

$$z_3 = z_1 + z_2$$

$$z_t = \sigma(z_3)$$

$$\textcircled{2}: z_4 = W_{rh} h_{t-1}$$

$$z_5 = W_{rx} x_t$$

$$z_6 = z_4 + z_5$$

$$r_t = \sigma(z_6)$$

$$\textcircled{3}: z_7 = r_t \odot h_{t-1}$$

$$z_8 = W_h \cdot z_7$$

$$z_9 = W_x x_t$$

$$z_{10} = z_8 + z_9$$

$$\tilde{h}_t = \tanh(z_{10})$$

$$\textcircled{4}: z_{11} = 1 - z_t$$

$$z_{12} = z_{11} \odot h_{t-1}$$

$$z_{13} = z_t \odot \tilde{h}_t$$

$$h_t = z_{12} + z_{13}$$

$$\nabla_{z_{12}} L = \nabla_{h_t} L$$

$$\nabla_{z_{13}} L = \nabla_{h_t} L$$

$$\nabla_{z_t} L = \nabla_{z_{13}} L \odot \tilde{h}_t^T$$

$$\nabla_{\tilde{h}_t} L = \nabla_{z_{13}} L \odot z_t^T$$

$$\nabla_{z_{11}} L = \nabla_{z_{12}} L \odot h_{t-1}^T$$

$$\nabla_{h_{t-1}} L = \nabla_{z_{12}} L \odot z_{11}^T$$

$$\nabla_{z_t} L += -\nabla_{z_{11}} L$$

$$\nabla_{z_{10}} L = \nabla_{\tilde{h}_t} L \odot (1 - \tanh^2(z_{10}))^T$$

$$\nabla_{z_6} L = \nabla_{r_t} L \odot \sigma'(z_6) \odot (1 - \sigma(z_6))^T$$

$$\nabla_{z_8} L = \nabla_{z_{10}} L$$

$$\nabla_{z_9} L = \nabla_{z_{10}} L$$

$$\nabla_{W_x} L = x_t (\nabla_{z_9} L)$$

$$\nabla_{x_t} L = (\nabla_{z_9} L) W_x$$

$$\nabla_{W_h} L = z_7 (\nabla_{z_8} L)$$

$$\nabla_{z_7} L = (\nabla_{z_8} L) W_h$$

$$\nabla_{r_t} L = (\nabla_{z_7} L) \odot h_{t-1}^T$$

$$\nabla_{h_{t-1}} L += (\nabla_{z_7} L) \odot r_t^T$$

$$\nabla_{z_4} L = \nabla_{z_6} L$$

$$\nabla_{z_5} L = \nabla_{z_6} L$$

$$\nabla_{W_{rx}} L = x_t (\nabla_{z_5} L)$$

$$\nabla_{x_t} L += (\nabla_{z_5} L) W_{rx}$$

$$\nabla_{W_{rh}} L = h_{t-1} (\nabla_{z_4} L)$$

$$\nabla_{h_{t-1}} L += (\nabla_{z_4} L) W_{rh}$$

$$\nabla_{z_3} L = \nabla_{z_t} L \circ \sigma(z_3 L)^T \circ (1 - \sigma(z_3 L))^T$$

$$\nabla_{z_2} L = \nabla_{z_3} L$$

$$\nabla_{z_1} L = \nabla_{z_3} L$$

$$\nabla_{W_{zx}} L = X_t (\nabla_{z_2} L)$$

$$\nabla_{X_t} L \leftarrow (\nabla_{z_2} L) W_{zx}$$

$$\nabla_{W_{zh}} L = h_{t-1} (\nabla_{z_1} L)$$

$$\nabla_{h_{t-1}} L \leftarrow (\nabla_{z_1} L) W_{zh}$$